lib/isabelle/State_monad_extras.thy
@@ -1,15 +1,22 @@
 theory State_monad_extras
-  imports State_monad
+  imports
+    State_monad
+    Sail_values_extras
+begin
+
+context
+  notes returnS_def[simp] and failS_def[simp] and throwS_def[simp] and readS_def[simp] and updateS_def[simp]
 begin
 
 abbreviation "bindS_aux f \<equiv> (\<lambda>r. case r of (Value a, s') \<Rightarrow> f a s' | (Ex e, s') \<Rightarrow> [(Ex e, s')])"
+abbreviation "bindS_app ms f \<equiv> List.concat (List.map (bindS_aux f) ms)"
 
 lemma bindS_ext_cong[fundef_cong]:
   assumes m: "m1 s = m2 s"
     and f: "\<And>a s'. (Value a, s') \<in> set (m2 s) \<Longrightarrow> f1 a s' = f2 a s'"
-  shows "(bindS m1 f1) s = (bindS m2 f2) s"
+  shows "bindS m1 f1 s = bindS m2 f2 s"
 proof -
-  have "List.concat (map (bindS_aux f1) (m2 s)) = List.concat (map (bindS_aux f2) (m2 s))"
+  have "bindS_app (m2 s) f1 = bindS_app (m2 s) f2"
     using f by (intro arg_cong[where f = List.concat]) (auto intro: map_ext split: result.splits)
   then show ?thesis using m by (auto simp: bindS_def)
 qed
@@ -20,8 +27,21 @@ lemma bindS_cong[fundef_cong]:
   shows "bindS m1 f1 = bindS m2 f2"
   using assms by (blast intro: bindS_ext_cong)
 
-lemma bindS_returnS[simp]: "bindS (returnS x) m = m x"
-  by (auto simp add: bindS_def returnS_def)
+lemma bindS_returnS_left[simp]: "bindS (returnS x) f = f x"
+  by (auto simp add: bindS_def)
+
+lemma bindS_returnS_right[simp]: "bindS m returnS = (m :: ('regs, 'a, 'e) monadS)"
+proof -
+  have "List.concat (map (bindS_aux returnS) ms) = ms" for ms :: "(('a, 'e) result \<times> 'regs sequential_state) list"
+    by (induction ms) (auto split: result.splits)
+  then show ?thesis unfolding bindS_def by blast
+qed
+
+lemma bindS_readS: "bindS (readS f) m = (\<lambda>s. m (f s) s)"
+  by (auto simp: bindS_def)
+
+lemma bindS_updateS: "bindS (updateS f) m = (\<lambda>s. m () (f s))"
+  by (auto simp: bindS_def)
 
 lemma bindS_assoc[simp]: "bindS (bindS m f) g = bindS m (\<lambda>x. bindS (f x) g)"
 proof -
@@ -31,13 +51,96 @@ proof -
   then show ?thesis unfolding bindS_def by auto
 qed
 
-lemma bindS_failS[simp]: "bindS (failS msg) f = failS msg" by (auto simp: bindS_def failS_def)
-lemma bindS_throwS[simp]: "bindS (throwS e) f = throwS e" by (auto simp: bindS_def throwS_def)
+lemma bindS_failS[simp]: "bindS (failS msg) f = failS msg" by (auto simp: bindS_def)
+lemma bindS_throwS[simp]: "bindS (throwS e) f = throwS e" by (auto simp: bindS_def)
 declare seqS_def[simp]
+
+lemma Value_bindS_elim:
+  assumes "(Value a, s') \<in> set (bindS m f s)"
+  obtains s'' a' where "(Value a', s'') \<in> set (m s)" and "(Value a, s') \<in> set (f a' s'')"
+  using assms by (auto simp: bindS_def; split result.splits; auto)
+
+abbreviation
+  "try_catchS_aux h r \<equiv>
+    (case r of
+       (Value a, s') => returnS a s'
+     | (Ex (Throw e), s') => h e s'
+     | (Ex (Failure msg), s') => [(Ex (Failure msg), s')])"
+abbreviation "try_catchS_app ms h \<equiv> List.concat (List.map (try_catchS_aux h) ms)"
 
 lemma try_catchS_returnS[simp]: "try_catchS (returnS a) h = returnS a"
   and try_catchS_failS[simp]: "try_catchS (failS msg) h = failS msg"
   and try_catchS_throwS[simp]: "try_catchS (throwS e) h = h e"
-  by (auto simp: returnS_def failS_def throwS_def try_catchS_def)
+  by (auto simp: try_catchS_def)
+
+lemma try_catchS_cong[cong]:
+  assumes "\<And>s. m1 s = m2 s" and "\<And>e s. h1 e s = h2 e s"
+  shows "try_catchS m1 h1 = try_catchS m2 h2"
+  using assms by (intro arg_cong2[where f = try_catchS] ext) auto
+
+fun ignore_throw_app :: "(('a, 'e1) result \<times> 's) list \<Rightarrow> (('a, 'e2) result \<times> 's) list" where
+  "ignore_throw_app [] = []"
+| "ignore_throw_app ((Value a, s) # ms) = (Value a, s) # ignore_throw_app ms"
+| "ignore_throw_app ((Ex (Failure msg), s) # ms) = (Ex (Failure msg), s) # ignore_throw_app ms"
+| "ignore_throw_app ((Ex (Throw e), s) # ms) = ignore_throw_app ms"
+abbreviation ignore_throw :: "('r, 'a, 'e1) monadS \<Rightarrow> ('r, 'a, 'e2) monadS" where
+  "ignore_throw m \<equiv> \<lambda>s. ignore_throw_app (m s)"
+
+lemma [simp]: "ignore_throw_app ms = (Ex (Throw e), s) # ms' \<longleftrightarrow> False"
+  by (induction ms rule: ignore_throw_app.induct) auto
+
+lemma ignore_throw_app_append[simp]:
+  "ignore_throw_app (ms1 @ ms2) = ignore_throw_app ms1 @ ignore_throw_app ms2"
+  by (induction ms1 rule: ignore_throw_app.induct) auto
+
+lemma ignore_throw_app_bindS_app[simp]:
+  "ignore_throw_app (bindS_app ms f) = bindS_app (ignore_throw_app ms) (ignore_throw \<circ> f)"
+  by (induction ms rule: ignore_throw_app.induct) (auto split: result.splits)
+
+lemma ignore_throw_bindS[simp]:
+  "ignore_throw (bindS m f) = bindS (ignore_throw m) (ignore_throw \<circ> f)"
+  "ignore_throw (bindS m f) s = bindS (ignore_throw m) (ignore_throw \<circ> f) s"
+  unfolding bindS_def by auto
+
+lemma try_catchS_bindS_no_throw:
+  fixes m1 :: "('r, 'a, 'e1) monadS" and m2 :: "('r, 'a, 'e2) monadS"
+  assumes m1: "\<And>s. ignore_throw m1 s = m1 s"
+    and m2: "\<And>s. ignore_throw m1 s = m2 s"
+  shows "try_catchS (bindS m1 f) h = bindS m2 (\<lambda>a. try_catchS (f a) h)"
+proof
+  fix s
+  have 1: "try_catchS_app (bindS_app ms f) h =
+        bindS_app (ignore_throw_app ms) (\<lambda>a s'. try_catchS_app (f a s') h)"
+    if "ignore_throw_app ms = ms" for ms
+    using that by (induction ms rule: ignore_throw_app.induct) auto
+  then show "try_catchS (bindS m1 f) h s = bindS m2 (\<lambda>a. try_catchS (f a) h) s"
+    using m1 unfolding try_catchS_def bindS_def m2[symmetric] by blast
+qed
+
+lemma no_throw_mem_builtins:
+  "\<And>a. ignore_throw (returnS a) = returnS a"
+  "\<And>BC rk a sz s. ignore_throw (read_mem_bytesS BC rk a sz) s = read_mem_bytesS BC rk a sz s"
+  "\<And>BC a s. ignore_throw (read_tagS BC a) s = read_tagS BC a s"
+  "\<And>BC wk a sz s. ignore_throw (write_mem_eaS BC wk a sz) s = write_mem_eaS BC wk a sz s"
+  "\<And>v s. ignore_throw (write_mem_bytesS v) s = write_mem_bytesS v s"
+  "\<And>BC v s. ignore_throw (write_mem_valS BC v) s = write_mem_valS BC v s"
+  "\<And>t s. ignore_throw (write_tagS t) s = write_tagS t s"
+  "\<And>s. ignore_throw (excl_resultS ()) s = excl_resultS () s"
+  unfolding read_mem_bytesS_def read_memS_def read_tagS_def write_mem_eaS_def write_mem_valS_def write_mem_bytesS_def write_tagS_def excl_resultS_def
+  by (auto simp: bindS_def chooseS_def Let_def split: option.splits)+
+
+lemma no_throw_read_memS: "ignore_throw (read_memS BCa BCb rk a sz) s = read_memS BCa BCb rk a sz s"
+  by (auto simp: read_memS_def no_throw_mem_builtins cong: bindS_cong)
+
+lemma no_throw_read_regvalS: "ignore_throw (read_regvalS r reg_name) s = read_regvalS r reg_name s"
+  by (cases r) (auto simp: bindS_def split: option.splits)
+
+lemma no_throw_write_regvalS: "ignore_throw (write_regvalS r reg_name v) s = write_regvalS r reg_name v s"
+  by (cases r) (auto simp: bindS_def split: option.splits)
+
+lemmas no_throw_builtins[simp, intro] =
+  no_throw_mem_builtins no_throw_read_regvalS no_throw_write_regvalS no_throw_read_memS
+
+end
 
 end
