lib/isabelle/Sail_values_extras.thy
@@ -1,0 +1,52 @@
+theory Sail_values_extras
+  imports Sail_values
+begin
+
+termination reverse_endianness_list by (lexicographic_order simp add: drop_list_def)
+
+termination index_list
+  by (relation "measure (\<lambda>(i, j, step). nat ((j - i + step) * sgn step))") auto
+
+lemma just_list_map_Some[simp]: "just_list (map Some v) = Some v" by (induction v) auto
+
+lemma just_list_None_iff[simp]: "just_list xs = None \<longleftrightarrow> None \<in> set xs"
+  by (induction xs) (auto split: option.splits)
+
+lemma just_list_Some_iff[simp]: "just_list xs = Some ys \<longleftrightarrow> xs = map Some ys"
+  by (induction xs arbitrary: ys) (auto split: option.splits)
+
+lemma just_list_cases:
+  assumes "just_list xs = y"
+  obtains (None) "None \<in> set xs" and "y = None"
+        | (Some) ys where "xs = map Some ys" and "y = Some ys"
+  using assms by (cases y) auto
+
+abbreviation "BC_bitU_list \<equiv> instance_Sail_values_Bitvector_list_dict instance_Sail_values_BitU_Sail_values_bitU_dict"
+lemmas BC_bitU_list_def = instance_Sail_values_Bitvector_list_dict_def instance_Sail_values_BitU_Sail_values_bitU_dict_def
+abbreviation "BC_mword \<equiv> instance_Sail_values_Bitvector_Machine_word_mword_dict"
+lemmas BC_mword_def = instance_Sail_values_Bitvector_Machine_word_mword_dict_def
+
+lemma image_bitU_of_bool_B0_B1: "bitU_of_bool ` bs \<subseteq> {B0, B1}"
+  by (auto simp: bitU_of_bool_def split: if_splits)
+
+lemma bool_of_bitU_bitU_of_bool[simp]: "bool_of_bitU \<circ> bitU_of_bool = id"
+  by (intro ext) (auto simp: bool_of_bitU_def bitU_of_bool_def)
+
+lemma nat_of_bits_aux_bl_to_bin_aux:
+  assumes "set bs \<subseteq> {B0, B1}"
+  shows "nat_of_bits_aux acc bs = nat (bl_to_bin_aux (map bool_of_bitU bs) (int acc))"
+  by (use assms in \<open>induction acc bs rule: nat_of_bits_aux.induct\<close>)
+     (auto simp: Bit_def bool_of_bitU_def intro!: arg_cong[where f = nat] arg_cong2[where f = bl_to_bin_aux])
+
+lemma nat_of_bits_bl_to_bin[simp]: "nat_of_bits (map bitU_of_bool bs) = nat (bl_to_bin bs)"
+  by (auto simp: nat_of_bits_def bl_to_bin_def nat_of_bits_aux_bl_to_bin_aux image_bitU_of_bool_B0_B1)
+
+lemma unsigned_bits_of_mword:
+  "unsigned_method BC_bitU_list (bits_of_method BC_mword a) = unsigned_method BC_mword a"
+  by (auto simp: BC_bitU_list_def BC_mword_def unsigned_of_bits_def)
+
+lemma unsigned_bits_of_bitU_list:
+  "unsigned_method BC_bitU_list (bits_of_method BC_bitU_list a) = unsigned_method BC_bitU_list a"
+  by (auto simp: BC_bitU_list_def)
+
+end
